partial_fun.lean
@@ -13,7 +13,17 @@ variable [decidable_eq α]
 
 -- Destructive addition to a context
 def extend (f : partial_fun α β) (x : α) (y : β) : partial_fun α β
-| x' := if x = x' then y else f x'
+| x' := if x' = x then y else f x'
 
 instance : has_insert (α × β) (partial_fun α β) :=
 ⟨λ ⟨a, b⟩ f, extend f a b⟩
+
+lemma extend_eta (f : partial_fun α β) (x : α) (y : β) :
+  extend f x y = λ x', if x' = x then y else f x' := rfl
+
+lemma extend_same (f : partial_fun α β) (x : α) (y : β) : extend f x y x = y :=
+by unfold extend; simp
+
+lemma extend_diff (f : partial_fun α β) {x x' : α} (y : β) :
+  x' ≠ x → extend f x y x' = f x' :=
+by intro h; unfold extend; simp [h]
