semantics.lean
@@ -11,16 +11,30 @@ inductive is_subst : term → term → term → var → Prop
 -- e = x{e/x}
 | same_var (x : var) (e : term) : is_subst e (term.var x) e x
 -- y = y{e/x}, y ≠ x
-| diff_var (x y : var) (e : term) : y ≠ x → is_subst (term.var y) (term.var y) e x
+| diff_var {x y : var} (e : term) : y ≠ x → is_subst (term.var y) (term.var y) e x
 -- e₁{e/x}e₂{e/x} = (e₁ e₂){e/x}
-| app (e₁ e₂ e₁' e₂' e : term) (x : var) :
+| app {e₁ e₂ e e₁' e₂' : term} {x : var} :
     is_subst e₁' e₁ e x → is_subst e₂' e₂ e x → is_subst (term.app e₁' e₂') (term.app e₁ e₂) e x
 -- λ y, e₁{e₂/x} = (λ y, e₁){e₂/x}, y ≠ x, y ∉ fv e₂
-| abs (y x : var) (e₁ e₁' e₂ : term) :
+| abs {x y : var} {e₁ e₂ e₁' : term} :
     y ≠ x → y ∉ fv e₂ → is_subst e₁' e₁ e₂ x → is_subst (term.abs y e₁') (term.abs y e₁) e₂ x
 
+def subst (e v : term) (x : var) : {e' // is_subst e' e v x} := sorry
+
 inductive step : term → term → Prop
-| context {e e' : term} {E : E} :
+| context {e e' : term} (E : E) :
     step e e' → step (E e) (E e')
-| beta (x : var) (e e' : term) (v : term)  :
+| beta {x : var} {e v e' : term}  :
     is_value v → is_subst e' e v x → step (term.app (term.abs x e) v) e'
+
+notation e `⇝` e' := step e e'
+
+-- reflexive transitive closure
+inductive rtc {α} (r : α → α → Prop) : α → α → Prop
+| refl  : ∀ {a}, rtc a a
+| trans : ∀ {a b c}, r a b → rtc b c → rtc a c
+
+def many_steps := rtc step
+notation e `⇝*` e' := many_steps e e'
+
+def halts e := ¬∃ e', step e e'
