soundness.lean
@@ -1,11 +1,12 @@
-import .typing
-import .semantics
+/-
+Soundness is typically proven by establishing progress and preservation
+-/
 
-def subst (e v : term) (x : var) : {e' // is_subst e' e v x} := sorry
+import .typing .semantics
 
 -- Hack: need to state Γ = ∅ since it will refuse to do induction directly on ∣- e : τ
 lemma progress {e : term} {τ : type} {Γ : ctx} :
-  Γ = emptyf → well_typed_under Γ e τ → is_value e ∨ ∃ e', step e e' :=
+  Γ = emptyf → well_typed_under Γ e τ → is_value e ∨ ∃ e', e ⇝ e' :=
 begin
   intros empty h,
   
@@ -23,7 +24,7 @@ begin
   { apply or.inl, apply is_value.abs },
 
   -- Applications always evaluate
-  case well_typed_under.app _ _ e₁ _ e₂ te₁ _ ih₁ ih₂
+  case well_typed_under.app _ e₁ e₂ _ _ te₁ _ ih₁ ih₂
   { apply or.inr,
     -- Apply the inductive hypothesis on e₁
     cases or.symm (ih₁ empty) with e₁_steps e₁_iv,
@@ -37,7 +38,7 @@ begin
     apply step.context, assumption,
 
     -- Apply the inductive hypothesis on e₂
-    cases or.symm (ih₂ empty) with e₂_steps e₂_iv,
+    cases or.symm (ih₂ empty) with e₂_steps,
 
     -- If the RHS steps, apply CONTEXT
     cases e₂_steps with e₂',
@@ -57,11 +58,101 @@ begin
     cases te₁ }
 end
 
+lemma well_typed_halts_is_value {e : term} {τ : type} : well_typed e τ → halts e → is_value e :=
+λ t, or.resolve_right (progress rfl t)
+
+lemma subst_lemma {x : var} {e e' es : term} {τ τ' : type} :
+  well_typed_under (extend emptyf x τ') e τ → well_typed e' τ' → is_subst es e e' x → well_typed es τ :=
+begin
+  intros te te' is,
+  induction is,
+
+  -- Trivial, since e is already well-typed
+  case is_subst.same_var
+  { cases te, simp at a,
+    injection a with h,
+    rw ←h, assumption },
+  
+  -- Impossible, the context doesn't have y
+  case is_subst.diff_var x _ _ h
+  { cases te,
+    rw [←extend_eta, extend_diff emptyf τ' h] at a,
+    contradiction },
+  
+  -- WTF
+  case is_subst.app _ _ _ _ _ x
+  { cases te,
+    rw ←extend_eta at a_3 a_2,
+    simp at a_3 a_2,
+    --let := ih_2 a_3,
+    admit,
+   },
+  
+  case is_subst.abs 
+  {
+      cases te,
+      rw ←extend_eta at a_3,
+      simp at a_3 a_2,
+      admit
+  }
+end
+
+lemma E_lemma {E : E} {e e' : term} {τ τ' : type} :
+  well_typed_under emptyf (E e) τ → well_typed_under emptyf e τ' → well_typed_under emptyf e' τ' →
+  well_typed (E e') τ :=
+begin
+  intros tEe te te',
+  --induction E,
+  --simp [show E.hole e = e, from rfl,show E.hole e' = e', from rfl] at *,
+  admit
+end
+
+lemma typing_hole {E : E} {e : term} {τ : type} :
+  well_typed (E e) τ → ∃ τ', well_typed e τ' :=
+begin
+  intro t,
+  induction E generalizing τ,
+
+  case E.hole
+  { existsi τ, assumption },
+
+  case E.app_left _ _ ih
+  { cases t, exact ih a_2 },
+
+  case E.app_right v _ ih
+  { cases v, cases t, exact ih a_2 }
+end
+
 lemma preservation {e e' : term} {τ : type} :
-  well_typed_under emptyf e τ → step e e' → well_typed_under emptyf e' τ :=
+  well_typed e τ → (e ⇝ e') → well_typed e' τ :=
 begin
   intros t s,
-  induction s with e e' E s ih,
-    admit,
-    admit
+  induction s generalizing τ,
+  
+  case step.beta
+  { cases t, cases a_2,
+    apply subst_lemma,
+    repeat { assumption } },
+  
+  case step.context _ _ _ _ ih
+  { cases typing_hole t with _ t',
+    let := ih t',
+    apply E_lemma,
+    repeat { assumption } },
+end
+
+theorem soundness {e e' : term} {τ : type} :
+  well_typed e τ → (e ⇝* e') → halts e' → is_value e' ∧ well_typed e' τ :=
+begin
+  intros t s h,
+  induction s,
+
+  case rtc.refl
+  { apply and.intro,
+    apply well_typed_halts_is_value,
+    repeat { assumption } },
+  
+  -- Ironically, the inductive step is easier...
+  case rtc.trans _ _ _ s _ ih
+  { exact ih (preservation t s) h }
 end
