typing.lean
@@ -1,5 +1,4 @@
-import .core
-import .partial_fun
+import .core .partial_fun
 
 def ctx := partial_fun var type
 
@@ -7,13 +6,14 @@ inductive well_typed_under : ctx → term → type → Prop
 | unit {Γ : ctx} :
     well_typed_under Γ term.unit type.unit
 
-| var {Γ : ctx} (x : var) (τ : type) :
+| var {Γ : ctx} {x : var} {τ : type} :
     Γ x = τ → well_typed_under Γ (term.var x) τ
 
-| abs {Γ : ctx} (x : var) (τ : type) (e : term) (τ' : type) :
+| abs {Γ : ctx} {x : var} {e : term} {τ τ' : type} :
     well_typed_under (extend Γ x τ) e τ' → well_typed_under Γ (term.abs x e) (type.func τ τ')
 
-| app {Γ : ctx} (τ : type) (e₁ : term) (τ' : type) (e₂ : term) :
+| app {Γ : ctx} {e₁ e₂ : term} {τ τ' : type} :
     well_typed_under Γ e₁ (type.func τ τ') → well_typed_under Γ e₂ τ →
       well_typed_under Γ (term.app e₁ e₂) τ'
 
+def well_typed := well_typed_under emptyf
